@prefix rdf:     <http://www.w3.org/1999/02/22-rdf-syntax-ns#> .
@prefix rdfs:    <http://www.w3.org/2000/01/rdf-schema#> .
@prefix telepathy:     <http://nepomuk.kde.org/ontologies/2009/06/20/telepathy#> .
@prefix nao:     <http://www.semanticdesktop.org/ontologies/2007/08/15/nao#> .
@prefix nrl:     <http://www.semanticdesktop.org/ontologies/2007/08/15/nrl#> .
@prefix nco:     <http://www.semanticdesktop.org/ontologies/2007/03/22/nco#> .
@prefix nie:     <http://www.semanticdesktop.org/ontologies/2007/01/19/nie#> .
@prefix xsd:     <http://www.w3.org/2001/XMLSchema#> .

telepathy: {telepathy:accountIdentifier
     a rdf:Property ;
          rdfs:subPropertyOf nao:identifier ;
          rdfs:comment "Identifier of a Local Telepathy Account (as given by the Telepathy Account Manager).";
          rdfs:domain nco:IMAccount ;
          rdfs:label "accountIdentifier" ;
          rdfs:range xsd:string ;
          nrl:maxCardinality "1".

            telepathy:statusType
     a rdf:Property ;
          rdfs:comment "The current presence type as defined by the Telepathy Spec. Invalid values (by the Telepathy spec) should be considered as 0, Unset.";
          rdfs:domain nco:IMAccount ;
          rdfs:label "statusType" ;
          rdfs:range xsd:integer ;
          nrl:maxCardinality "1" .

            telepathy:avatar
     a rdf:Property ;
          rdfs:comment "The photo which is the IM Account's avatar. This is a special case of the nco:photo property of the parent nco:personContact." ;
          rdfs:domain nco:IMAccount ;
          rdfs:label "avatar" ;
          rdfs:range nie:DataObject ;
          nrl:maxCardinality "1" .
}

<http://nepomuk.kde.org/ontologies/2009/06/20/telepathy/metadata>
{
    telepathy:
          a       nrl:DocumentGraph , nrl:Ontology ;
          nao:hasDefaultNamespace "http://nepomuk.kde.org/ontologies/2009/06/20/telepathy#" ;
          nao:hasDefaultNamespaceAbbreviation "telepathy" ;
          nao:lastModified "2009-06-20T20:46:32.866Z" ;
          nao:serializationLanguage "TriG" ;
          nao:status "Testing" ;
          nrl:updatable "0" ;
          nao:version "1" .

    <http://nepomuk.kde.org/ontologies/2009/06/20/telepathy/metadata>
          a       nrl:GraphMetadata , nrl:Ontology ;
          nao:serializationLanguage "TriG" ;
          nrl:coreGraphMetadataFor telepathy: .
}
